First working version

tests/lean/run/structuralOverNested.lean
@@ -1,121 +1,68 @@
+inductive Tree where | node : List Tree → Tree
+
+mutual
+def Tree.size : Tree → Nat
+  | node ts => list_size ts
+
+def Tree.list_size : List Tree → Nat
+  | [] => 0
+  | t::ts => t.size + list_size ts
+end
+
+example : Tree.list_size (t :: ts) = t.size + Tree.list_size ts := rfl
+
 
 -- A nested inductive type
--- the `Unit → Tree α` prevents well-founded recursion
+-- the `Bool → RTree α` prevents well-founded recursion and
+-- tests support for reflexive types
 
-inductive Tree (α : Type u) : Type u
- | node : α → (Bool → Tree α) → List (Tree α) → Tree α
-
+inductive RTree (α : Type u) : Type u
+ | node : α → (Bool → RTree α) → List (RTree α) → RTree α
 
 -- only recurse on the non-nested component
-def Tree.simple_size : Tree α → Nat
+def RTree.simple_size : RTree α → Nat
   | .node _x t _ts => 1 + (t true).simple_size + (t false).simple_size
 
 /--
-info: theorem Tree.simple_size.eq_1.{u_1} : ∀ {α : Type u_1} (_x : α) (t : Bool → Tree α) (_ts : List (Tree α)),
-  (Tree.node _x t _ts).simple_size = 1 + (t true).simple_size + (t false).simple_size :=
-fun {α} _x t _ts => Eq.refl (Tree.node _x t _ts).simple_size
+info: theorem RTree.simple_size.eq_1.{u_1} : ∀ {α : Type u_1} (_x : α) (t : Bool → RTree α) (_ts : List (RTree α)),
+  (RTree.node _x t _ts).simple_size = 1 + (t true).simple_size + (t false).simple_size :=
+fun {α} _x t _ts => Eq.refl (RTree.node _x t _ts).simple_size
 -/
 #guard_msgs in
-#print Tree.simple_size.eq_1
+#print RTree.simple_size.eq_1
+
+-- set_option trace.Elab.definition.structural true
 
 -- also recurse on the nested components
-/--
-error: fail to show termination for
-  Tree.size
-  Tree.aux_size
-with errors
-failed to infer structural recursion:
-Not considering parameter α of Tree.size:
-  it is unchanged in the recursive calls
-Not considering parameter α of Tree.aux_size:
-  it is unchanged in the recursive calls
-Skipping arguments of type Tree α, as Tree.aux_size has no compatible argument.
-Skipping arguments of type List (Tree α), as Tree.size has no compatible argument.
-
-
-Could not find a decreasing measure.
-The arguments relate at each recursive call as follows:
-(<, ≤, =: relation proved, ? all proofs failed, _: no proof attempted)
-Call from Tree.size to Tree.size at 25:24-37:
- #1
-  ?
-Call from Tree.size to Tree.size at 25:40-54:
- #1
-  _
-Call from Tree.size to Tree.aux_size at 25:57-68:
-   #1
-#2  _
-Call from Tree.aux_size to Tree.size at 28:13-19:
-   #2
-#1  _
-Call from Tree.aux_size to Tree.aux_size at 28:22-33:
- #2
-  _
-
-
-#1: sizeOf x1
-#2: sizeOf x1
-
-Please use `termination_by` to specify a decreasing measure.
--/
 #guard_msgs in
 mutual
-def Tree.size : Tree α → Nat
+def RTree.size : RTree α → Nat
   | .node _ t ts => 1 + (t true).size + (t false).size + aux_size ts
-def Tree.aux_size : List (Tree α) → Nat
+def RTree.aux_size : List (RTree α) → Nat
   | [] => 0
   | t::ts => t.size + aux_size ts
 end
 
 /--
-error: fail to show termination for
-  Tree.map
-  Tree.map_aux
-with errors
-failed to infer structural recursion:
-Not considering parameter α of Tree.map:
-  it is unchanged in the recursive calls
-Not considering parameter β of Tree.map:
-  it is unchanged in the recursive calls
-Not considering parameter f of Tree.map:
-  it is unchanged in the recursive calls
-Not considering parameter α of Tree.map_aux:
-  it is unchanged in the recursive calls
-Not considering parameter β of Tree.map_aux:
-  it is unchanged in the recursive calls
-Not considering parameter f of Tree.map_aux:
-  it is unchanged in the recursive calls
-Skipping arguments of type Tree α, as Tree.map_aux has no compatible argument.
-Skipping arguments of type List (Tree α), as Tree.map has no compatible argument.
-
-
-Could not find a decreasing measure.
-The arguments relate at each recursive call as follows:
-(<, ≤, =: relation proved, ? all proofs failed, _: no proof attempted)
-Call from Tree.map to Tree.map at 73:42-53:
- #1
-  ?
-Call from Tree.map to Tree.map_aux at 73:56-68:
-   #1
-#2  _
-Call from Tree.map_aux to Tree.map at 76:13-20:
-   #2
-#1  _
-Call from Tree.map_aux to Tree.map_aux at 76:24-36:
- #2
-  _
-
-
-#1: sizeOf x1
-#2: sizeOf x1
-
-Please use `termination_by` to specify a decreasing measure.
+info: theorem RTree.aux_size.eq_2.{u_1} : ∀ {α : Type u_1} (t : RTree α) (ts : List (RTree α)),
+  RTree.aux_size (t :: ts) = t.size + RTree.aux_size ts :=
+fun {α} t ts => Eq.refl (RTree.aux_size (t :: ts))
 -/
 #guard_msgs in
+#print RTree.aux_size.eq_2
+
 mutual
-def Tree.map (f : α → β) : Tree α → Tree β
+def RTree.map (f : α → β) : RTree α → RTree β
   | .node x t ts => .node (f x) (fun b => (t b).map f) (map_aux f ts)
-def Tree.map_aux (f : α → β) : List (Tree α) → List (Tree β)
+def RTree.map_aux (f : α → β) : List (RTree α) → List (RTree β)
   | [] => []
   | t::ts => t.map f :: map_aux f ts
 end
+
+/--
+info: theorem RTree.map_aux.eq_2.{u_1, u_2} : ∀ {α : Type u_1} {β : Type u_2} (f : α → β) (t : RTree α) (ts : List (RTree α)),
+  RTree.map_aux f (t :: ts) = RTree.map f t :: RTree.map_aux f ts :=
+fun {α} {β} f t ts => Eq.refl (RTree.map_aux f (t :: ts))
+-/
+#guard_msgs in
+#print RTree.map_aux.eq_2
