src/Lean/Elab/PreDefinition/Structural/IndGroupInst.lean
@@ -1,0 +1,79 @@
+/-
+Copyright (c) 2024 Lean FRO. All rights reserved.
+Released under Apache 2.0 license as described in the file LICENSE.
+Authors: Joachim Breitner
+-/
+prelude
+import Lean.Elab.PreDefinition.Structural.Basic
+import Lean.Meta.InferType
+
+namespace Lean.Elab.Structural
+open Lean Meta
+
+/--
+An instance of an mutually inductive group of inductives, identified by the `all` array
+and the level and expressions parameters.
+
+For example this distinguishes between `List α` and `List β` and we will not even attempt
+mutual structural recursion on such incompatible types.
+-/
+structure IndGroupInst where
+  all       : Array Name
+  levels    : List Level
+  params    : Array Expr
+  numNested : Nat
+
+
+def IndGroupInst.ofRecArgInfo (recArgInfo : RecArgInfo) : IndGroupInst :=
+  { all := recArgInfo.indAll
+    levels := recArgInfo.indLevels
+    params := recArgInfo.indParams
+    numNested := recArgInfo.indNumNested
+  }
+
+def IndGroupInst.toMessageData (igi : IndGroupInst) : MessageData :=
+  mkAppN (.const igi.all[0]! igi.levels) igi.params
+
+instance : ToMessageData IndGroupInst where
+  toMessageData := IndGroupInst.toMessageData
+
+def IndGroupInst.numMotives (igi : IndGroupInst) : Nat :=
+  igi.all.size + igi.numNested
+
+def IndGroupInst.isDefEq (igi1 igi2 : IndGroupInst) : MetaM Bool := do
+  unless igi1.all[0]! = igi2.all[0]! do return false
+  unless igi1.levels.length = igi2.levels.length do return false
+  unless (igi1.levels.zip igi2.levels).all (fun (l₁, l₂) => Level.isEquiv l₁ l₂) do return false
+  unless igi1.params.size = igi2.params.size do return false
+  unless (← (igi1.params.zip igi2.params).allM (fun (e₁, e₂) => Meta.isDefEqGuarded e₁ e₂)) do return false
+  return true
+
+/--
+Figures out the nested type formers of an inductive group, with parameters instantiated
+and indices still forall-abstracted.
+
+For example given a nested inductive
+```
+inductive Tree α where | node : α → Vector (Tree α) n → Tree α
+```
+(where `n` is an index of `Vector`) and the instantiation `Tree Int` it will return
+```
+#[(n : Nat) → Vector (Tree Int) n]
+```
+
+-/
+def IndGroupInst.nestedTypeFormers (igi : IndGroupInst) : MetaM (Array Expr) := do
+  if igi.numNested = 0 then return #[]
+  -- We extract this information from the motives of the recursor
+  let recName := mkRecName igi.all[0]!
+  let recInfo ← getConstInfoRec recName
+  assert! recInfo.numMotives = igi.numMotives
+  let aux := mkAppN (.const recName (0 :: igi.levels)) igi.params
+  let motives ← inferArgumentTypesN recInfo.numMotives aux
+  let auxMotives : Array Expr := motives[igi.all.size:]
+  auxMotives.mapM fun motive =>
+    forallTelescopeReducing motive fun xs _ => do
+      assert! xs.size > 0
+      mkForallFVars xs.pop (← inferType xs.back)
+
+end Lean.Elab.Structural
